\documentclass[a4paper,11pt]{article}

% Import packages
\usepackage[a4paper]{geometry}
\usepackage[utf8]{inputenc}
\usepackage{amsmath}
\usepackage{amssymb}
\usepackage{bussproofs}
\usepackage{proof}

% Change enumerate environments you use letters
\renewcommand{\theenumi}{\alph{enumi}}

\title{Peergrade assignment 1}
\author{Author: Kristoffer HÃ¸jelse} 
\date{\today}

\begin{document} 

\maketitle

\section*{Exercise 1}

\subsection*{1.1. Prove in natural deduction...}

$$
\infer[ \to I^{h_1} ]{ (\neg A \lor \neg B) \to (C \to (A \land B)) \to \neg C }{
    \infer[ \to I^{h_2} ]{ (C \to (A \land B)) \to \neg C }{
        \infer[ \neg I^{h_3} ]{ \neg C }{
            \infer[\neg E]{ \bot }{
                \infer[\neg i^{h_4}]{ \neg ( A \land B) }{
                    \infer[ \lor e^{h_5 , h_6} ]{\bot}{
                        \infer[h_1]{\neg A \lor \neg B}{}
                        &
                        \infer[\neg e]{\bot}{
                            \infer[h_5]{\neg A}{}
                            &
                            \infer[\land e_1]{A}{
                                \infer[h_4]{A \land B}{}
                            }
                        }
                        &
                        \infer[\neg e]{\bot}{
                            \infer[h_6]{\neg B}{}
                            &
                            \infer[\land e_1]{B}{
                                \infer[h_4]{A \land B}{}
                            }
                        }
                    }
                }
                &
                \infer[\to E]{A \land B}{
                    \infer[h_3]{C}{}
                    &
                    \infer[h_2]{C \to A \land B}{}
                }
            }
        }
    }
}
$$

Note: at $\neg i^{h_4}$ the proof for De Morgan's Law begins, the equivalence of:

$$\neg(A \land B) \equiv (\neg A \lor \neg B) $$

\subsection*{1.2. Construct a truth table...}

\begin{center}
\begin{tabular}{ |c c c| c | c c | c }
 A & B & C & $\neg C$ & $A \land B$ & $ C \to (A \land B) $ & $ (C \to (A \land B)) \to \neg C $ \\ 
 T & T & T & F & T & T & F \\  
 T & T & F & T & T & T & T \\
 T & F & T & F & F & F & T \\
 T & F & F & T & F & T & T \\
 F & T & T & F & F & F & T \\
 F & T & F & T & F & T & T \\
 F & F & T & F & F & F & T \\
 F & F & F & T & F & T & T \\
\end{tabular}
\end{center}

\begin{center}
\begin{tabular}{ c c c | c }
 $ \neg A $ & $ \neg B $ & $ \neg A \lor \neg B $ & $ (\neg A \lor \neg B) \to (C \to (A \land B)) \to \neg C $ \\ 
 F & F & F & T \\  
 F & F & F & T \\
 F & T & T & T \\
 F & T & T & T \\
 T & F & T & T \\
 T & F & T & T \\
 T & T & T & T \\
 T & T & T & T \\
\end{tabular}
\end{center}

It seems that $ (\neg A \lor \neg B) \to (C \to (A \land B)) \to \neg C $ is a Tautology.

$$ \bold{T} \equiv (\neg A \lor \neg B) \to (C \to (A \land B)) \to \neg C $$

\newpage
\section*{Exercise 2}
\subsection*{2.1}
Expression using quantifiers

T = table, L = has legs
\begin{equation}
    \exists x(T(x) \to \neg L(x))
\end{equation}
Negation of the statement

T = table, L = has legs
\begin{equation}
    \forall x(T(x) \to L(x))
\end{equation}
Expression using English

For all x,
if x is a table
then x has legs.

\subsection*{2.2}
Expression using quantifiers

E = Even
\begin{equation}
    \forall x \in Z(E(x) \to \exists y \in Z((y = x^{2}) \to E(y))
\end{equation}
Negation of the statement

E = Even

\begin{equation}
    \exists x \in Z(E(x) \to \exists y \in Z((y = x^{2}) \to \neg E(y))
\end{equation}
Expression using English

There exists an x in the domain of all integers,
if x is an even integer
then there exists a y in the domain of all integers,
if y is equal to the square of x,
then y is NOT an even integer.

\subsection*{2.3}
Expression using quantifiers

H = Is a house, P = Has pink doors

\begin{equation}
    \exists x ( H(x) \to P(x) )
\end{equation}
Negation of the statement

H = Is a house, P = Has pink doors
\begin{equation}
    \forall x (H(x) \to \neg P(x))
\end{equation}
Expression using English

For all x,
if x is a house
then x does not have pink doors.

\subsection*{2.4}
Expression using quantifiers

P = Is a part of "the pigs", F = Can fly, D = Can dance

\begin{equation}
    \forall x( P(x) \to F(x) \land D(x) )
\end{equation}
Negation of the statement

P = Is a part of "the pigs", F = Can fly, D = Can dance
\begin{equation}
    \exists x( P(x) \to \neg (F(x) \land D(x)) )
\end{equation}
Expression using English

There exists an x where,
if x is a part of "the pigs"
then x can not fly and dance.

\subsection*{2.5}
Expression using quantifiers

Q = Rational

\begin{equation}
    \exists x \left( Q(x) \to \sqrt{Q(x)} = 2 \right)
\end{equation}
Negation of the statement

Q = Rational
\begin{equation}
    \forall x \left( Q(x) \to \sqrt{Q(x)} \neq 2 \right)
\end{equation}
Expression using English

For all x,
if x is a rational number
then the square root of x is not equal to 2.

\newpage
\section*{Exercise 3}
\subsection*{Prove in natural deduction...}

$$
\infer[\to I^{h_1}]{\forall x (A(x) \to B(x)) \to \exists y (\neg B(y)) \to \neg \forall z (A(z))}{
    \infer[\to I^{h_2}]{\exists y (\neg B(y)) \to \neg \forall z (A(z))}{
        \infer[\neg I^{h_3}]{\forall z (A(z))}{
            \infer[\neg e]{\bot}{
                \infer[\exists e^{h_4}]{\neg B(a)}{
                    \infer[h_2]{\exists y (\neg B(y))}{}
                    &
                    \infer[\neg e]{\neg B(a)}{
                        \infer[h_4]{\neg B(y)}{}
                        &
                        \infer[\to e]{B(y)}{
                            \infer[\forall e]{A(y) \to B(y)}{
                                \infer[h_1]{\forall x (A(x) \to B(x))}{}
                            }
                            &
                            \infer[\forall e]{A(y)}{
                                \infer[h_3]{\forall z (A(z))}{}
                            }
                        }
                    }
                }
                &
                \infer[]{B(a)}{
                    \infer[\forall e]{A(a) \to B(a)}{
                        \infer[h_1]{\forall x (A(x) \to B(x))}{}
                    }
                    &
                    \infer[\forall e]{A(a)}{
                        \infer[h_3]{\forall z (A(z))}{}
                    }
                }
            }
        }
    }
}
$$

\end{document}
